isabelle/SubstContext.thy
@@ -9,36 +9,104 @@ fun (sequential) depthECE :: "ece \<Rightarrow> nat" where
 | "depthECE (CAppr _ _) = 1"
 | "depthECE _ = 0"
 
-fun depthEC :: "ec \<Rightarrow> nat" where
+definition depthEC :: "ec \<Rightarrow> nat" where
   "depthEC ec = sum_list (map depthECE ec)"
 
+lemma depthECE_isXE[simp]: "isXE ece \<Longrightarrow> depthECE ece = 0"
+  by (induction ece) (auto elim: isXE.cases)
+
+lemma depthEC_isX[simp]: "isX ec \<Longrightarrow> depthEC ec = 0"
+  by (induction ec) (auto simp add: isX_def depthEC_def)
+
+fun substVCE :: "nat \<Rightarrow> val \<Rightarrow> vce \<Rightarrow> vce" where
+  "substVCE n v (CTup vs1 vs2) = CTup (map (substV n v) vs1) (map (substV n v) vs2)"
+
+definition substVC :: "nat \<Rightarrow> val \<Rightarrow> vc \<Rightarrow> vc" where
+  "substVC n v vc = map (substVCE n v) vc"
+
+fun substECE :: "nat \<Rightarrow> val \<Rightarrow> ece \<Rightarrow> ece" where
+  "substECE n v (CVal vc) = CVal (substVC n v vc)"
+| "substECE n v CDef = CDef"
+| "substECE n v (CAppl vc v2) = CAppl (substVC n v vc) (substV n v v2)"
+| "substECE n v (CAppr v1 vc) = CAppr (substV n v v1) (substVC n v vc)"
+| "substECE n v (CSeql e2) = CSeql (substE n v e2)"
+| "substECE n v (CSeqr e1) = CSeqr (substE n v e1)"
+| "substECE n v (CBarl e2) = CBarl (substE n v e2)"
+| "substECE n v (CBarr e1) = CBarr (substE n v e1)"
+| "substECE n v (CUnil e2) = CUnil (substE n v e2)"
+| "substECE n v (CUnir e1) = CUnir (substE n v e1)"
+| "substECE n v COne = COne"
+| "substECE n v CAll = CAll"
+
+fun substEC :: "nat \<Rightarrow> val \<Rightarrow> ec \<Rightarrow> ec" where
+  "substEC n v [] = []" 
+| "substEC n v (ece#ec) = substECE n v ece # substEC (depthECE ece + n) (\<up>\<^sub>v (depthECE ece) 0 v) ec" 
+
+lemma depthECE_substECE[simp]: "depthECE (substECE n v ece) = depthECE ece"
+  by (induction ece) auto
+
+lemma depthEC_substEC[simp]: "depthEC (substEC n v ec) = depthEC ec"
+  by (induction ec arbitrary: n v) (auto simp add: depthEC_def)
+
+
 definition "occursVCE n vce = occursV n (appVCE vce (Const 0))"
+
+definition occursVC where "occursVC n vc \<longleftrightarrow> (\<exists> vce \<in> set vc. occursVCE n vce)"
+
+lemma occursVC_Nil[simp]: "occursVC n [] = False"
+  by (simp add: occursVC_def appVC_def appVC'_def)
+
+lemma occursVC_Cons[simp]: "occursVC n (vce # vc) = occursVCE n vce \<or> occursVC n vc"
+  by (auto simp add: occursVC_def appVC_def appVC'_def)
+
+definition "occursECE n ece = occursE n (appECE ece Fail)"
+
+fun occursEC where
+  "occursEC n [] = False"
+| "occursEC n (ece # ec) \<longleftrightarrow> occursECE n ece \<or> occursEC (depthECE ece + n) ec"
 
 lemma occursV_appVCE[simp]:
   "occursV n (appVCE vce v) \<longleftrightarrow> occursV n v \<or> occursVCE n vce"
   by (cases vce) (auto simp add: occursVCE_def)
 
-definition "occursVC n vc = occursV n (appVC vc Fail)"
-
 lemma occursE_appVC[simp]:
   "occursV n (appVC vc e) \<longleftrightarrow> occursE (1 + n) e \<or> occursVC n vc"
   by (induction vc) (auto simp add: appVC_def appVC'_def occursVC_def)
-
-definition "occursECE n ece = occursE n (appECE ece Fail)"
 
 lemma occursE_appECE[simp]:
   "occursE n (appECE ece e) \<longleftrightarrow> occursE (depthECE ece + n) e \<or> occursECE n ece"
   by (cases ece) (auto simp add: occursECE_def)
 
-definition "occursEC n ec = occursE n (appEC ec Fail)"
-
 lemma occursE_appEC[simp]:
   "occursE n (appEC ec e) \<longleftrightarrow> occursE (depthEC ec + n) e \<or> occursEC n ec "
-  apply (induction ec arbitrary: n)
-   apply (auto simp add: appEC_def occursEC_def simp del: occursE_appECE)
-  apply (metis ab_semigroup_add_class.add_ac(1) group_cancel.add2 occursE_appECE)
+  apply (induction n ec rule: occursEC.induct)
+   apply (auto simp add: appEC_def depthEC_def)
+  apply (metis ab_semigroup_add_class.add_ac(1) group_cancel.add2)
   apply (simp add: ab_semigroup_add_class.add_ac(1) add.commute)
-  apply simp
   done
+
+lemma occursVCE_substVCE[simp]:
+  "occursVCE i (substVCE n v vce) \<longleftrightarrow> 
+  (i \<noteq> n \<and> occursVCE i vce) \<or> (occursVCE n vce \<and> occursV i v)"
+  apply (induction vce)
+  apply (auto simp add: occursVCE_def )
+  apply (meson Un_iff imageI occursV_substV)+
+  done
+
+lemma occursVC_substVC[simp]:
+  "occursVC i (substVC n v vc) \<longleftrightarrow> 
+  (i \<noteq> n \<and> occursVC i vc) \<or> (occursVC n vc \<and> occursV i v)"
+  by (auto simp add: substVC_def occursVC_def)
+
+lemma occursECE_substECE[simp]:
+  "occursECE i (substECE n v ece) \<longleftrightarrow> 
+  (i \<noteq> n \<and> occursECE i ece) \<or> (occursECE n ece \<and> occursV i v)"
+  by (cases ece) (auto simp add: occursECE_def)
+
+
+lemma occursEC_substEC[simp]:
+  "occursEC i (substEC n v ec) \<longleftrightarrow> 
+  (i \<noteq> n \<and> occursEC i ec) \<or> (occursEC n ec \<and> occursV i v)"
+  by (induction ec arbitrary: i n v) (auto simp add: occursV_liftV)
 
 end
